@prefix identity: <http://BreeAnn7.github.io/skos_example/> .
@prefix dct: <http://purl.org/dc/terms/> .
@prefix skos: <http://www.w3.org/2004/02/skos/core#> .
@prefix xsd: <http://www.w3.org/2001/XMLSchema#> .
@prefix aat: <http://vocab.getty.edu/aat/> .

identity: a skos:ConceptScheme ;
    dct:title "Identity Terminology Schema"@en ;
    skos:prefLabel "Identity Terminology Schema" ;
    dct:creator "Bree Midavaine"@en ;
    dct:created "2021-12-13"^^xsd:date ;
    dct:license <https://creativecommons.org/publicdomain/zero/1.0/> ;
    skos:hasTopConcept identity:a0001, identity:a0002, identity:a0003, identity:a0004, identity:a0005 .

identity:a0001 a skos:Concept ;
    skos:prefLabel "Ability Status"@en ;
    skos:definition "Referring to whether or not someone has a disability, physical or mental. (NCDJ)"@en ;
	skos:narrower identity:a0006 ;
	skos:narrower identity:a0007 ;
	skos:scopeNote "Do not use for tagging or annotation."@en ;
    skos:topConceptOf identity: .

identity:a0002 a skos:Concept ;
    skos:prefLabel "Ethnic Identities"@en ;
    skos:definition "One way in which a group of people identify themselves as part of a larger group based on ancestral origin and/or skin color. Ethnicity, like race, is a socially constructed idea. (Incluseum)"@en ;
	skos:narrower identity:a0011 ;
	skos:scopeNote "Do not use for tagging or annotation."@en ;
    skos:topConceptOf identity: .  

identity:a0003 a skos:Concept ;
    skos:prefLabel "Gender Identities"@en ;
    skos:definition "An individual’s feeling about, relationship with, and understanding of gender as it pertains to their sense of self. An individual’s gender identity may or may not be related to the sex that individual was assigned at birth. (NCTE)"@en ;
	skos:scopeNote "Do not use for tagging or annotation."@en ;
    skos:topConceptOf identity: .  

identity:a0004 a skos:Concept ;
    skos:prefLabel "Sexual Identities"@en ;
    skos:definition "An inherent or immutable enduring emotional, romantic, or sexual attraction to other people. (term: Incluseum/definition: HRC)"@en ;
	skos:scopeNote "Do not use for tagging or annotation."@en ;
    skos:topConceptOf identity: .  

identity:a0005 a skos:Concept ;
    skos:prefLabel "Religious Identities"@en ;
    skos:definition "An individual’s association with particular belief systems that encompass various personal and institutional relationships between human beings and what they regard as holy, sacred, or divine, usually but not always a deity, or a spiritual or occult force. (Getty)"@en ;
	skos:scopeNote "Do not use for tagging or annotation."@en ;
    skos:topConceptOf identity: . 

identity:a0006 a skos:Concept ;
    skos:prefLabel "Non-disabled"@en ;
	skos:hiddenLabel "Abled"@en ;
	skos:hiddenLabel "Able-bodied"@en ;
    skos:definition "A person who does not identify as having a disability. (NCDJ)"@en ;
	skos:scopeNote "Do not use the terms Abled or Able-bodied."@en ;
	skos:broader identity:a0001 ;
  	skos:inScheme identity: .
    
identity:a0007 a skos:Concept ;
    skos:prefLabel "Neurodiverse"@en ;
    skos:definition "The range of differences in individual brain function and behavioral traits, regarded as part of the normal variation in the human population. (NCDJ)"@en ;
	skos:scopeNote "Do not use for tagging or annotation. This is an umbrella term which should NOT be assigned to either groups of people or an individual person."@en ;
	skos:broader identity:a0001 ;
	skos:narrower identity:a0008 ;
	skos:narrower identity:a0009 ;
    skos:inScheme identity: .

identity:a0008 a skos:Concept ;
    skos:prefLabel "Neurotypical"@en ;
    skos:definition "A person who is considered part of the normal variation in the human population (NCDJ)"@en ;
	skos:broader identity:a0007 ;
    skos:inScheme identity: .

identity:a0009 a skos:Concept ;
    skos:prefLabel "Neurodivergent"@en ;
	skos:altLabel "Neuroatypical"@en ;
    skos:definition "A person who is considered part of the normal variation in the human population (NCDJ)"@en ;
	skos:broader identity:a0007 ;
	skos:narrower identity:a0010 ;
    skos:inScheme identity: .

identity:a0010 a skos:Concept ;
    skos:prefLabel "Autistic spectrum disorder"@en ;
    skos:definition "An umbrella term for a group of complex disorders related to brain development."@en ;
	skos:scopeNote "(NCDJ) Opinions vary on how to refer to someone with autism. Some people with autism prefer being referred to as “autistic” or an “autistic person.” Others object to using autistic as an adjective. The Autism Self Advocacy Network details this debate.  NCDJ recommendation is to refer to someone as having autistic spectrum disorder only if the information is relevant to the story and you are confident there is a medical diagnosis. Ask individuals how they prefer to be described."@en ;
	skos:broader identity:a0009 ;
    skos:inScheme identity: .

identity:a0011 a skos:Concept ;
    skos:prefLabel "BIPOC"@en ;
    skos:definition "A blanket term for Black, Indigenous, people of color. May also be used by those who identify as Black, Indigenous, or a person of color to show solidarity with other racial or ethnic groups who have been marginalized."@en ;
	skos:scopeNote "This is an umbrella term which should not be assigned to either groups of people or an individual person. Refer to the specific group if possible. e.g. First Nations, African American"@en ;
	skos:broader identity:a0002 ;
	skos:narrower identity:a0012 ;
    skos:inScheme identity: .

identity:a0012 a skos:Concept ;
    skos:prefLabel "Asian"@en ;
    skos:definition "A term as broad as European. In American usage, Asian is generally used to refer to the entire continent of Asia; often, however, Asian is used as shorthand for East Asians, or East and Southeast Asians. (DSG) People living in a general region which encompasses China, India, Indonesia, Bangladesh, Japan, Korea, Philippines, Vietnam, Thailand, Taiwan, Cambodia, Hong Kong, Singapore."@en ;
	skos:scopeNote "This is an umbrella term which should not be assigned to either groups of people or an individual person. Refer to the specific nationality if possible."@en ;
	skos:broader identity:a0010 ;
	skos:narrower identity:a0013 ;
	skos:narrower identity:a0014 ;
    skos:inScheme identity: .

identity:a0013 a skos:Concept ;
    skos:prefLabel "AAPI"@en ;
	skos:altLabel "Asian American and Pacific Islander"@en ;
	skos:definition "Acronym for Asian American and Pacific Islander."@en ;
    skos:scopeNote "This is an umbrella term which should not be assigned to either groups of people or an individual person. Refer to the specific nationality if possible."@en ;
	skos:broader identity:a0012 ;
    skos:inScheme identity: .

identity:a0014 a skos:Concept ;
    skos:prefLabel "Asian American"@en ;
	skos:definition "Americans of Asian descent in North America. (Getty)"@en ;
	skos:scopeNote "Do not hyphenate. When possible, ask people how they identify (Asian American, Chinese American, Japanese American, etc…)"@en ;
	skos:exactMatch aat:300385962 ;
	skos:broader identity:a0012 ;
    skos:inScheme identity: .